@prefix dcterms: <http://purl.org/dc/terms/> .
@prefix mav: <http://cadmiumkitty.github.io/moneyaggvoc/> .
@prefix rdf: <http://www.w3.org/1999/02/22-rdf-syntax-ns#> .
@prefix rdfs: <http://www.w3.org/2000/01/rdf-schema#> .
@prefix skos: <http://www.w3.org/2004/02/skos/core#> .
@prefix xml: <http://www.w3.org/XML/1998/namespace> .
@prefix xsd: <http://www.w3.org/2001/XMLSchema#> .

mav:mav003 a skos:Concept ;
    dcterms:source <https://www.ecb.europa.eu/stats/money_credit_banking/monetary_aggregates/html/hist_content.en.html> ;
    skos:altLabel "Narrow money" ;
    skos:broader mav:mav002 ;
    skos:definition "Narrow money (M1) includes currency, i.e. banknotes and coins, as well as balances which can immediately be converted into currency or used for cashless payments, i.e. overnight deposits." ;
    skos:inScheme mav:scheme ;
    skos:prefLabel "M1" .

mav:mav004 a skos:Concept ;
    dcterms:source <https://www.ecb.europa.eu/stats/money_credit_banking/monetary_aggregates/html/hist_content.en.html> ;
    skos:altLabel "Intermediate money" ;
    skos:broader mav:mav002 ;
    skos:definition "Intermediate money (M2) comprises narrow money (M1) and, in addition, deposits with a maturity of up to two years and deposits redeemable at a period of notice of up to three months. Depending on their degree of moneyness, such deposits can be converted into components of narrow money, but in some cases there may be restrictions involved, such as the need for advance notification, delays, penalties or fees. The definition of M2 reflects the particular interest in analysing and monitoring a monetary aggregate that, in addition to currency, consists of deposits which are liquid." ;
    skos:inScheme mav:scheme ;
    skos:prefLabel "M2" .

mav:mav007 a skos:Concept ;
    dcterms:source <https://www.federalreserve.gov/faqs/money_12845.htm> ;
    skos:broader mav:mav006 ;
    skos:definition "The monetary base is defined as the sum of currency in circulation and reserve balances (deposits held by banks and other depository institutions in their accounts at the Federal Reserve)." ;
    skos:inScheme mav:scheme ;
    skos:note "This measure is not listed in Economics CFA Program Curriculum 2016 Level I Volume 2 Reading 19 Exhibit 3 Definitions of Money (ISBN 978-1-942471-19-6)" ;
    skos:prefLabel "Monetary base" .

mav:mav008 a skos:Concept ;
    dcterms:source <https://www.federalreserve.gov/faqs/money_12845.htm> ;
    skos:broader mav:mav006 ;
    skos:definition "M1 is defined as the sum of currency held by the public and transaction deposits at depository institutions (which are financial institutions that obtain their funds mainly through deposits from the public, such as commercial banks, savings and loan associations, savings banks, and credit unions)." ;
    skos:inScheme mav:scheme ;
    skos:prefLabel "M1" .

mav:mav009 a skos:Concept ;
    dcterms:source <https://www.federalreserve.gov/faqs/money_12845.htm> ;
    skos:broader mav:mav006 ;
    skos:definition "M2 is defined as M1 plus savings deposits, small-denomination time deposits (those issued in amounts of less than $100,000), and retail money market mutual fund shares." ;
    skos:inScheme mav:scheme ;
    skos:prefLabel "M2" .

mav:mav011 a skos:Concept ;
    dcterms:source <http://www.boj.or.jp/en/statistics/outline/exp/data/exms01.pdf> ;
    skos:broader mav:mav010 ;
    skos:definition "Currency in circulation + deposit money deposited at depository institutions." ;
    skos:inScheme mav:scheme ;
    skos:prefLabel "M1" .

mav:mav012 a skos:Concept ;
    dcterms:source <http://www.boj.or.jp/en/statistics/outline/exp/data/exms01.pdf> ;
    skos:broader mav:mav010 ;
    skos:definition "Currency in circulation + deposits deposited at domestically licensed banks, etc. (\"domestically licensed banks, etc.\" indicates the same range of financial institutions stipulated as \"M2+CDs depository institutions\" in the former statistics)." ;
    skos:inScheme mav:scheme ;
    skos:prefLabel "M2" .

mav:mav013 a skos:Concept ;
    dcterms:source <http://www.boj.or.jp/en/statistics/outline/exp/data/exms01.pdf> ;
    skos:broader mav:mav010 ;
    skos:definition "Currency in circulation + deposits deposited at depository institutions." ;
    skos:inScheme mav:scheme ;
    skos:prefLabel "M3" .

mav:mav014 a skos:Concept ;
    dcterms:source <http://www.boj.or.jp/en/statistics/outline/exp/data/exms01.pdf> ;
    skos:broader mav:mav010 ;
    skos:definition "M3 + pecuniary trusts + investment trusts + bank debentures + straight bonds issued by banks + commercial paper issued by financial institutions + government securities + foreign bonds." ;
    skos:inScheme mav:scheme ;
    skos:note "This measure is not listed in Economics CFA Program Curriculum 2016 Level I Volume 2 Reading 19 Exhibit 3 Definitions of Money (ISBN 978-1-942471-19-6)" ;
    skos:prefLabel "L" .

mav:mav016 a skos:Concept ;
    dcterms:source <https://www.bankofengland.co.uk/statistics/details/further-details-about-m0-data> ;
    skos:broader mav:mav015 ;
    skos:definition """M0 comprised sterling notes and coin in circulation outside the Bank of England (including those held in banks' and building societies' tills), and banks’ operational deposits with the Bank of England.
 
M0 data differ from M4 and other balance sheet statistics because they were compiled as a monthly average of weekly observations. They also included all notes and coin in circulation, whereas M4 only includes those held by the non-bank non-building society private sector. """ ;
    skos:inScheme mav:scheme ;
    skos:prefLabel "M0" .

mav:mav017 a skos:Concept ;
    dcterms:source <https://www.bankofengland.co.uk/statistics/details/further-details-about-m4-data> ;
    skos:altLabel "Retail M4" ;
    skos:broader mav:mav015 ;
    skos:definition """Retail M4 (or M2) comprises:

The M4 private sector's
holdings of sterling notes and coin; and
sterling denominated 'retail' deposits with UK MFIs.
As noted in the August 1992 Quarterly Bulletin (page 317), the definition of the deposits which, along with notes and coin, previously comprised M2 was altered with effect from the flow for December 1992.

Retail deposits are defined as deposits which arise from a customer's acceptance of an advertised rate (including nil) for a particular product, typically 'retail' deposits are taken in the reporters' branch networks. With effect from October 2007, there was a change in the treatment of non-interest bearing deposits (see Valuation and Breaks).

Acceptances
The treatment of bank acceptances changed in September 1997, and was backdated. Acceptances are still being reported off balance sheet by individual reporters, but in the aggregated accounts and monetary statistics they count as on balance sheet of the accepting reporters (i.e. reporters accepting a bill are regarded as having a liability to the bill's owner and a claim on the party whose bill has been accepted).

Other MFI deposits include all Tax Exempt Special Savings Accounts (TESSAs) (until maturity in April 2004) and (cash) Individual Savings Accounts (ISAs).
Repos include sale and repurchase agreements against marketable securities of all kinds. An institution selling a security under a repo retains the security on its balance sheet and records a liability to the counterparty representing the cash received. Thus, a repo is a kind of secured deposit. The matching asset will depend on how the cash proceeds were employed. An institution acquiring a security under a reverse repo does not include the security on its balance sheet but records a claim on the counterparty representing the funds lent. The matching liability will depend on how the loan is funded.""" ;
    skos:inScheme mav:scheme ;
    skos:prefLabel "M2" .

mav:mav018 a skos:Concept ;
    dcterms:source <https://www.bankofengland.co.uk/statistics/details/further-details-about-m4-data> ;
    skos:broader mav:mav015 ;
    skos:definition """M4 comprises:

The M4 private sector's (i.e. the UK private sector other than monetary financial institutions (MFIs)) holdings of: 
sterling notes and coin;
sterling deposits, including certificates of deposit; 
commercial paper, bonds, FRNs and other instruments of up to and including five years' original maturity issued by UK MFIs;
claims on UK MFIs arising from repos (from December 1995);
estimated holdings of sterling bank bills;

and

35% of the sterling inter-MFI difference (added to OFC deposits, within wholesale M4). For further details please see the September 2011 Statistics article ‘Estimation and allocation methods within money and credit data’. Prior to September 2011, 95% of the domestic sterling interbank (now inter-MFI) difference was allocated to OFC deposits, the remaining 5% being allocated to transits. This followed a review of its causes (see page 101 of the June 1992 Economic Trends).
The sectoral distribution of holdings of CDs cannot be fully identified; errors may affect M4 itself, as well as its sectoral analysis.

Seasonally adjusted quarterly M4 is calculated as households' M4 (seasonally adjusted) plus PNFCs' M4 (seasonally adjusted) plus OFCs M4 (seasonally adjusted). More details are available in the Statistics article Seasonal adjustment of quarterly M4 excluding intermediate OFCs (M4ex) published in September 2010. Following a review of the seasonal adjustment method for non-intermediate OFCs once a sufficient run of monthly data was available, changes were made to the seasonally adjusted measures of M4 and M4 lending to bring them into line with the usual approach. The changes are detailed in the October 2013 Statistics article, ‘Modifications to the seasonally adjusted measures of M4 and M4 lending excluding intermediate OFCs’. """ ;
    skos:inScheme mav:scheme ;
    skos:prefLabel "M4" .

mav:mav019 a skos:Concept ;
    dcterms:source <https://www.bankofengland.co.uk/statistics/details/further-details-about-m3-estimate-of-european-monetary-union-aggregate-for-the-uk> ;
    skos:broader mav:mav015 ;
    skos:definition """The European Central Bank's broad monetary aggregate is M3. This encompasses also two narrower aggregates, M1 and M2.

Euro-area M3 is made up of monetary liabilities of euro-area monetary financial institutions (MFIs) and central government (Debt Management Office) vis-à-vis non-MFI euro-area residents excluding central government, in all currencies:

currency in circulation (M1)
overnight deposits (M1)
deposits with agreed maturity up to two years (M2)
deposits redeemable at notice up to three months (M2)
repurchase agreements
money market fund shares/units and money market paper
debt securities up to two years.
The estimate of M3 we compile for the UK is made up of monetary liabilities of MFIs in the UK vis-à-vis non-MFI UK residents excluding central government, in all currencies. The UK reporting system does not currently identify the maturity breakdowns used in the euro-area definition. These are therefore estimated.

The euro-area aggregate does not include the adjustments for transit items and the inter-MFI reporting difference, which are made for UK M4. A reconciliation table which illustrates the differences between M4 and this estimate of M3 is available on request.

These data therefore provide an estimate of M3 for the UK. These data replaced the M3H European harmonised aggregate, which was previously published to facilitate international comparisons between EU member states.

M3H comprised the components of M4 plus:

foreign currency deposits held by the M4 private sector with MFIs in the UK
sterling and foreign currency deposits held by UK public corporations with MFIs in the UK.
For further information on the compilation of these aggregates see the Statistics article 'Euro area monetary aggregates and their role in the Eurosystem's monetary policy strategy' in the ECB's Monthly Bulletin.""" ;
    skos:inScheme mav:scheme ;
    skos:prefLabel "M3H" ;
    skos:related mav:mav005 .

mav:mav005 a skos:Concept ;
    dcterms:source <https://www.ecb.europa.eu/stats/money_credit_banking/monetary_aggregates/html/hist_content.en.html> ;
    skos:altLabel "Broad money" ;
    skos:broader mav:mav002 ;
    skos:definition "Broad money (M3) comprises M2 and marketable instruments issued by the MFI sector. Certain money market instruments, in particular money market fund (MMF) shares/units and repurchase agreements are included in this aggregate. A high degree of liquidity and price certainty make these instruments close substitutes for deposits. As a result of their inclusion, M3 is less affected by substitution between various liquid asset categories than narrower definitions of money, and is therefore more stable." ;
    skos:inScheme mav:scheme ;
    skos:prefLabel "M3" .

mav:mav002 a skos:Concept ;
    dcterms:source <https://www.ecb.europa.eu/stats/money_credit_banking/monetary_aggregates/html/hist_content.en.html> ;
    skos:broader mav:mav001 ;
    skos:definition """The ECB's definition of euro area monetary aggregates is based on the following:
A harmonised definition of the money-issuing sector. It consists of those entities which issue liabilities with a high degree of moneyness to non-MFIs located in the euro area (excluding central government). This sector comprises MFIs resident in the euro area.
A harmonised definition of the money-holding sector, which comprises all non-MFIs resident in the euro area (except central government). In addition to households, non-financial corporations and financial institutions which are not MFIs are included, as well as state and local governments and social security funds. Central governments are considered to constitute a "money-neutral" sector, with one exception: central government liabilities with a monetary character (Post Office accounts, national savings accounts and Treasury accounts) are included as a special item in the definition of monetary aggregates.
The harmonised definitions of MFI liabilities categories. These make it possible to distinguish between MFI liabilities according to their degree of moneyness, while also taking into account the features of different financial systems.""" ;
    skos:exactMatch <http://eurovoc.europa.eu/1825> ;
    skos:inScheme mav:scheme ;
    skos:prefLabel "Eurozone money aggregate" .

mav:mav006 a skos:Concept ;
    dcterms:source <https://www.federalreserve.gov/faqs/money_12845.htm> ;
    skos:broader mav:mav001 ;
    skos:definition "The money supply is commonly defined to be a group of safe assets that households and businesses can use to make payments or to hold as short-term investments. For example, U.S. currency and balances held in checking accounts and savings accounts are included in many measures of the money supply." ;
    skos:inScheme mav:scheme ;
    skos:prefLabel "Unites States money aggregate" .

mav:mav010 a skos:Concept ;
    dcterms:source <http://www.boj.or.jp/en/statistics/outline/exp/data/exms01.pdf> ;
    skos:altLabel "Japan money stock statistics" ;
    skos:broader mav:mav001 ;
    skos:definition "The Money Stock Statistics (MSS) records the aggregate amount of money, including currency in circulation and deposit money, held by money holders such as non-financial corporations, individuals, and local governments." ;
    skos:inScheme mav:scheme ;
    skos:prefLabel "Japan money aggregate" .

mav:mav015 a skos:Concept ;
    skos:broader mav:mav001 ;
    skos:inScheme mav:scheme ;
    skos:prefLabel "United Kingdom money aggregate" .

mav:mav001 a skos:Concept ;
    dcterms:source <http://dbpedia.org/resource/Money_supply> ;
    skos:definition "In economics, the money supply or money stock, is the total amount of monetary assets available in an economy at a specific time. There are several ways to define \"money\", but standard measures usually include currency in circulation and demand deposits (depositors' easily accessed assets on the books of financial institutions)." ;
    skos:inScheme mav:scheme ;
    skos:prefLabel "Money aggregate" .

mav:scheme a skos:ConceptScheme ;
    rdfs:label "Money Aggregate Vocabulary" ;
    dcterms:creator <https://www.linkedin.com/in/emorozov/> ;
    rdfs:comment "Money Aggregate Vocabulary, or MoneyAggVoc for short, is an attempt to catalogue money aggregate measures listed in the Exhibit 3 Definitions of Money in Reading 19 on Economics of the CFA Program Curriculum 2016 Level I (ISBN 978-1-942471-19-6) with some minor additions. Although the CFA Program Curriculum inspired the structure of the information in this vocabulary, the actual content was taken from the open sources (DBpedia, Federal Reserve System, European Central Bank, Bank of Japan and Bank of England) and includes appropriate references." ;
    skos:hasTopConcept mav:mav001 .

